add L2 semantics

LeanScratch/Semantics/L2/Red.lean
@@ -16,10 +16,10 @@ inductive Red : State → State → Prop
   | op1 : Red ⟨e, s⟩ ⟨e', s'⟩
       → Red ⟨.op e o e2, s⟩ ⟨.op e' o e2, s'⟩
   | op2 : Red ⟨e2, s⟩ ⟨e2', s'⟩
-      → e.isInt → Red ⟨.op e o e2, s⟩ ⟨.op e o e2', s'⟩
+      → e.IsValue → Red ⟨.op e o e2, s⟩ ⟨.op e o e2', s'⟩
 
   | deref : (h : s.lookup addr = some x)
-      → Red ⟨.deref (addr), s⟩ ⟨.int x, s⟩
+      → Red ⟨.deref addr, s⟩ ⟨.int x, s⟩
   | assign1 : (h : ∃ x, s.lookup addr = some x)
       → Red ⟨.assign addr (.int v), s⟩ ⟨.skip, s.insert addr v⟩
   | assign2 : Red ⟨e, s⟩ ⟨e', s'⟩ → Red ⟨.assign addr e, s⟩ ⟨.assign addr e', s'⟩
@@ -36,182 +36,83 @@ inductive Red : State → State → Prop
 
   | ewhile : Red ⟨.ewhile c body, stx⟩ ⟨.eif c (.seq body (.ewhile c body)) .skip, stx⟩
 
-  | beta : repl.isFnValue
-      → Red ⟨.app (.abs name _ body) repl, s⟩ ⟨body.subst name repl, s⟩
   | app1 : Red ⟨e1, s⟩ ⟨e1', s'⟩
       → Red ⟨.app e1 e2, s⟩ ⟨.app e1' e2, s'⟩
-  | app2 : e1.isFnValue → Red ⟨e2, s⟩ ⟨e2', s'⟩
+  | app2 : e1.IsValue → Red ⟨e2, s⟩ ⟨e2', s'⟩
       → Red ⟨.app e1 e2, s⟩ ⟨.app e1 e2', s'⟩
+  | fn : repl.IsValue
+      → Red ⟨.app (.abs t body) repl, s⟩ ⟨body.β repl, s⟩
 
--- copy pasted from l1
-@[simp]
-theorem skip_op_int : Red ⟨.op (.skip) o e, s⟩ ⟨sta, stx⟩ → False := by
-  intro h
-  cases h
-  <;> contradiction
+  | let1 : Red ⟨e1, s1⟩ ⟨e2, s2⟩
+      → Red ⟨.letVal t e1 e, s1⟩ ⟨.letVal t e2 e, s2⟩
+  | let2 : e1.IsValue
+      → Red ⟨.letVal t e1 e, s1⟩ ⟨e.β e1, s1⟩
+  -- TODO: add this
+  /- | letrecfn : -/
+  /-       Red ⟨.letRecVal (.arrow t1 t2) (.abs t1 e1) e2, s⟩ ⟨e2.β (.abs) , s⟩ -/
 
-@[simp]
-theorem seq1_simp : Red ⟨.seq .skip e, s⟩ ⟨stx, sta⟩ → Red ⟨.seq .skip e, s⟩ ⟨e, s⟩ := fun _ => .seq1
+/- theorem red_det : Red i o₁ ∧ Red i o₂ → o₁ = o₂ := by -/
+/-   intro ⟨ha, hb⟩ -/
+/-   induction ha generalizing o₂ -/
+/-   <;> cases hb -/
+/-   <;> try trivial -/
 
-@[simp]
-theorem seq1_simp' : Red ⟨.seq .skip e, s⟩ ⟨stx, sta⟩ → stx = e ∧ s = sta := by
-  intro h
-  cases h
-  · exact ⟨rfl, rfl⟩
-  · contradiction
+/-   case op1.op2 epre spre e₁ s₁ op eprealt ha a_ih e₂ s₂ epre_is_int hb =>  -/
+/-     rw [p] at ha -/
+/-     contradiction -/
 
-@[simp]
-theorem if_t_simp : Red ⟨.eif (.bool true) e1 e2, s⟩ ⟨stx, sta⟩ → Red ⟨.eif (.bool true) e1 e2, s⟩ ⟨e1, s⟩ := fun _ => .if_t
+/-   case op2.op1 epre spre e₁ s₁ e op ha e_is_int a_ih e₂ s₂ hb => -/
+/-     have ⟨_, p⟩ := isInt_defn.mpr e_is_int -/
+/-     rw [p] at hb -/
+/-     contradiction -/
 
-@[simp]
-theorem if_f_simp : Red ⟨.eif (.bool false) e1 e2, s⟩ ⟨stx, sta⟩ → Red ⟨.eif (.bool false) e1 e2, s⟩ ⟨e2, s⟩ := fun _ => .if_f
+/-   case op1.op1 epre spre e₁ s₁ o e2 ha a_ih e₂ s₂ hb => -/
+/-     injection a_ih hb with eq₁ eq₂ -/
+/-     rw [eq₁, eq₂] -/
+/-   case op2.op2 epre spre e₁ s₁ _ op ha epre_is_int a_ih e₂ s₂ _ hb => -/
+/-     injection a_ih hb with eq₁ eq₂ -/
+/-     rw [eq₁, eq₂] -/
 
-@[simp]
-theorem assign_simp : Red ⟨.assign addr e, s⟩ ⟨stx, sta⟩ → (∃ e', ∃ s', Red ⟨e, s⟩ ⟨e', s'⟩ ∧ stx = .assign addr e' ∧ sta = s') ∨ (stx = .skip) := by
-  intro h
-  cases h
-  · right
-    rfl
-  case assign2 e'2 a =>
-    left
-    use e'2
-    use sta
+/-   case deref.deref h₁ _ h₂=> -/
+/-     injection h₁.symm.trans h₂ with eq₁ -/
+/-     rw [eq₁] -/
 
-@[simp]
-theorem deref_simp : Red ⟨.deref addr, s⟩ ⟨stx, sta⟩ → (∃ i, stx = .int i) ∧ sta = s := by
-  intro h
-  cases h
-  case deref x h =>
-    constructor
-    · use x
-    · rfl
+/-   case assign2.assign2 epre spre e₁ s₁ addr ha a_ih e₂ s₂ hb => -/
+/-     injection a_ih hb with eq₁ eq₂ -/
+/-     rw [eq₁, eq₂] -/
 
-@[simp]
-theorem skip_simp : Red ⟨.skip, s⟩ ⟨stx, sta⟩ ↔ False := by
-  constructor
-  <;> intro h
-  · cases h
-  · contradiction
+/-   case seq2.seq2 epre spre e₁ s₁ erhs ha a_ih e₂ s₂ hb => -/
+/-     injection a_ih hb with eq₁ eq₂ -/
+/-     rw [eq₁, eq₂] -/
 
-@[simp]
-theorem bool_simp : Red ⟨.bool b, s⟩ ⟨stx, sta⟩ ↔ False := by
-  constructor
-  <;> intro h
-  · cases h
-  · contradiction
+/-   case if_cond.if_cond condpre spre cond₁ s₁ e1 e2 ha a_ih cond₂ s₂ hb =>  -/
+/-     injection a_ih hb with eq₁ eq₂ -/
+/-     rw [eq₁, eq₂] -/
 
-@[simp]
-theorem int_simp : Red ⟨.int b, s⟩ ⟨stx, sta⟩ ↔ False := by
-  constructor
-  <;> intro h
-  · cases h
-  · contradiction
+/-   case beta.app2 x name body repl s replVal _ _ _ a  => -/
+/-     cases repl -/
+/-     <;> simp only at replVal -/
+/-     <;> cases a -/
+/-   case app1.app1 e s e₁ s₁ e₂ s₂ a_ih e₁' s₁' a => -/
+/-     injection a_ih a with eq₁ eq₂ -/
+/-     rw [eq₁, eq₂] -/
+/-   case app1.app2 e _ _ _ _ a _ _ _ v _ => -/
+/-     cases e -/
+/-     <;> simp only at v -/
+/-     <;> cases a -/
 
+/-   case app2.beta e _ _ _ a _ _ _ _ _ v => -/
+/-     cases e -/
+/-     <;> simp only at v -/
+/-     <;> cases a -/
 
-@[simp]
-theorem abs_simp : Red ⟨.abs nm ty body, s⟩ ⟨stx, sta⟩ ↔ False := by
-  constructor
-  <;> intro h
-  · cases h
-  · contradiction
+/-   case app2.app1 e v _ _ _ _ a => -/
+/-     cases e -/
+/-     <;> simp only at v -/
+/-     <;> cases a -/
+/-   case app2.app2 e s e₁ s₁ e' e'v _ a_ih _ _ _ a => -/
+/-     injection a_ih a with eq₁ eq₂ -/
+/-     rw [eq₁, eq₂] -/
 
-@[simp]
-theorem op_add_simp : Red ⟨.op (.int a) .add (.int b), s⟩ ⟨stx, sta⟩ → Red ⟨.op (.int a) .add (.int b), s⟩ ⟨.int (a + b), s⟩ := by
-  intro h
-  cases h <;> try trivial
-  exact .op_add a b
-
-@[simp]
-theorem bool_op_int : Red ⟨.op (.bool b) o e, s⟩ ⟨sta, stx⟩ → False := by
-  intro h
-  cases h
-  <;> contradiction
-
-@[simp]
-theorem op_elim : Red ⟨.op lhs o rhs, s⟩ ⟨post, s'⟩ → (
-  if let .add := o then ∃ i, post = Expr.int i else ∃ b, post = Expr.bool b
-) ∨ (∃ l, ∃ r, post = .op l o r) := by
-  intro h
-  cases h
-  case op_add a b =>
-    left
-    use a + b
-  case op_gte a b =>
-    left
-    simp only [ge_iff_le, Expr.bool.injEq, exists_const]
-    use a >= b
-  case op1 e' _ =>
-    right
-    use e'
-    use rhs
-  case op2 e2' _ _ =>
-    right
-    use lhs
-    use e2'
-
-theorem red_det : Red i o₁ ∧ Red i o₂ → o₁ = o₂ := by
-  intro ⟨ha, hb⟩
-  induction ha generalizing o₂
-  <;> cases hb
-  <;> try trivial
-
-  case op1.op2 epre spre e₁ s₁ op eprealt ha a_ih e₂ s₂ epre_is_int hb => 
-    have ⟨_, p⟩ := isInt_defn.mpr epre_is_int
-    rw [p] at ha
-    contradiction
-
-  case op2.op1 epre spre e₁ s₁ e op ha e_is_int a_ih e₂ s₂ hb =>
-    have ⟨_, p⟩ := isInt_defn.mpr e_is_int
-    rw [p] at hb
-    contradiction
-
-  case op1.op1 epre spre e₁ s₁ o e2 ha a_ih e₂ s₂ hb =>
-    injection a_ih hb with eq₁ eq₂
-    rw [eq₁, eq₂]
-  case op2.op2 epre spre e₁ s₁ _ op ha epre_is_int a_ih e₂ s₂ _ hb =>
-    injection a_ih hb with eq₁ eq₂
-    rw [eq₁, eq₂]
-
-  case deref.deref h₁ _ h₂=>
-    injection h₁.symm.trans h₂ with eq₁
-    rw [eq₁]
-
-  case assign2.assign2 epre spre e₁ s₁ addr ha a_ih e₂ s₂ hb =>
-    injection a_ih hb with eq₁ eq₂
-    rw [eq₁, eq₂]
-
-  case seq2.seq2 epre spre e₁ s₁ erhs ha a_ih e₂ s₂ hb =>
-    injection a_ih hb with eq₁ eq₂
-    rw [eq₁, eq₂]
-
-  case if_cond.if_cond condpre spre cond₁ s₁ e1 e2 ha a_ih cond₂ s₂ hb => 
-    injection a_ih hb with eq₁ eq₂
-    rw [eq₁, eq₂]
-
-  case beta.app2 x name body repl s replVal _ _ _ a  =>
-    cases repl
-    <;> simp only at replVal
-    <;> cases a
-  case app1.app1 e s e₁ s₁ e₂ s₂ a_ih e₁' s₁' a =>
-    injection a_ih a with eq₁ eq₂
-    rw [eq₁, eq₂]
-  case app1.app2 e _ _ _ _ a _ _ _ v _ =>
-    cases e
-    <;> simp only at v
-    <;> cases a
-
-  case app2.beta e _ _ _ a _ _ _ _ _ v =>
-    cases e
-    <;> simp only at v
-    <;> cases a
-
-  case app2.app1 e v _ _ _ _ a =>
-    cases e
-    <;> simp only at v
-    <;> cases a
-  case app2.app2 e s e₁ s₁ e' e'v _ a_ih _ _ _ a =>
-    injection a_ih a with eq₁ eq₂
-    rw [eq₁, eq₂]
-
-end L2
+/- end L2 -/
 
