LeanScratch/Semantics/L2/Stx.lean
@@ -35,7 +35,61 @@ inductive Expr
   | abs (ty : Ty) (body : Expr)
   | app (fn arg : Expr) ---------> inference is decidable this is not needed
                         -- FUN!: Implement unification and make this nicer
+  | letVal (t : Ty) (val body : Expr)
+  | letRecVal (t : Ty) (val body : Expr)
 deriving DecidableEq, Repr
 
-end L2
+namespace Expr
+
+inductive IsValue : Expr → Prop
+  | bool : IsValue (.bool b)
+  | int : IsValue (.int i)
+  | skip : IsValue .skip
+  | fn : IsValue (.abs ty body)
+
+def bvarShift (shift skip : ℕ) : Expr → Expr
+  | .bvar n => .bvar $ if n < skip then n else n + shift
+  | .abs ty body => .abs ty (body.bvarShift shift skip.succ)
+  | .letVal t val body =>
+    .letVal    t (val.bvarShift shift skip     ) (body.bvarShift shift skip.succ)
+  | .letRecVal t val body =>
+    .letRecVal t (val.bvarShift shift skip.succ) (body.bvarShift shift skip.succ)
+
+  | .app a b => .app (a.bvarShift shift skip) (b.bvarShift shift skip)
+  | .seq a b => .seq (a.bvarShift shift skip) (b.bvarShift shift skip)
+  | .assign addr body => .assign addr (body.bvarShift shift skip)
+  | .ewhile c body => .ewhile (c.bvarShift shift skip) (body.bvarShift shift skip)
+  | .eif c t f => .eif (c.bvarShift shift skip) (t.bvarShift shift skip) (f.bvarShift shift skip)
+  | .op a o b => .op (a.bvarShift shift skip) o (b.bvarShift shift skip)
+  | x@(.deref _)
+  | x@(.skip)
+  | x@(.int _)
+  | x@(.bool _) => x
+
+def replace.bvar (bvarId idx_shift : ℕ) (replace : Expr) : Expr :=
+  match compare bvarId idx_shift with
+  | .lt => .bvar bvarId
+  | .eq => replace.bvarShift idx_shift 0
+  | .gt => .bvar bvarId.pred
+
+def replace (idx_shift : ℕ) (body repl : Expr) : Expr := match body with
+  | .bvar n => replace.bvar n idx_shift repl
+  | .abs ty body => .abs ty (body.replace idx_shift.succ repl)
+  | .letVal t val body =>
+    .letVal    t (val.replace idx_shift      repl) (body.replace idx_shift.succ repl)
+  | .letRecVal t val body =>
+    .letRecVal t (val.replace idx_shift.succ repl) (body.replace idx_shift.succ repl)
+
+  | .app a b => .app (a.replace idx_shift repl) (b.replace idx_shift repl)
+  | .seq a b => .seq (a.replace idx_shift repl) (b.replace idx_shift repl)
+  | .assign addr body => .assign addr (body.replace idx_shift repl)
+  | .ewhile c body => .ewhile (c.replace idx_shift repl) (body.replace idx_shift repl)
+  | .eif c t f => .eif (c.replace idx_shift repl) (t.replace idx_shift repl) (f.replace idx_shift repl)
+  | .op a o b => .op (a.replace idx_shift repl) o (b.replace idx_shift repl)
+  | x@(.deref _)
+  | x@(.skip)
+  | x@(.int _)
+  | x@(.bool _) => x
+
+def β : Expr → Expr → Expr := replace 0
 
