LeanScratch/Semantics/L2/Supo2.lean
@@ -1,0 +1,300 @@
+import LeanScratch.Semantics.L2.Stx
+import LeanScratch.Semantics.L2.Red
+import LeanScratch.Semantics.L2.Typed
+
+namespace L2
+
+section Q19
+
+inductive Expr.FV : Expr → ℕ → Prop
+  | opl : FV lhs n → FV (.op lhs o rhs) n
+  | opr : FV rhs n → FV (.op lhs o rhs) n
+
+  | eifc : FV c n → FV (.eif c t f) n
+  | eift : FV t n → FV (.eif c t f) n
+  | eiff : FV f n → FV (.eif c t f) n
+
+  | assign : FV e n → FV (.assign addr e) n
+
+  | seqa : FV a n → FV (.seq a b) n
+  | seqb : FV b n → FV (.seq a b) n
+
+  | appfn  : FV a n → FV (.app a b) n
+  | apparg : FV b n → FV (.app a b) n
+
+  | bvar : FV (.bvar idx) idx
+  | abs : FV body n.succ → FV (.abs t body) n
+  | letValVal : FV val n      → FV (.letVal t val _) n
+  | letValIn  : FV vin n.succ → FV (.letVal t _ vin) n
+  | letRecValVal : FV val n.succ → FV (.letRecVal t val _) n
+  | letRecValIn  : FV vin n.succ → FV (.letRecVal t _ vin) n
+
+abbrev Ex1 := (Expr.op (.bvar 0) .add (.app (.abs .int (.bvar 2)) (.int 2)))
+abbrev Ex1.Set : Set ℕ := {0, 1}
+
+-- cant be bothered to show the iff
+theorem Ex1.P : ∀ x ∈ Ex1.Set, Ex1.FV x :=
+  fun x hx => by
+    rcases hx with (hx|hx) <;> simp_all only [Set.mem_singleton_iff]
+    · exact .opl .bvar
+    · exact .opr $ .appfn $ .abs $ .bvar
+
+abbrev Ex2 := (Expr.op (.bvar 0) .add (.abs .int (.bvar 2)))
+abbrev Ex2.Set : Set ℕ := {0, 1}
+
+theorem Ex2.P : ∀ x ∈ Ex2.Set, Ex2.FV x :=
+  fun x hx => by
+    rcases hx with (hx|hx) <;> simp_all only [Set.mem_singleton_iff]
+    · exact .opl .bvar
+    · exact .opr $ .abs $ .bvar
+
+abbrev Ex3 := (Expr.abs .int $ .abs .int $ .abs .int $ .bvar 0)
+
+theorem Ex3.P : ∀ n, ¬Ex3.FV n :=
+  fun x hx => by
+    cases hx; rename_i hx
+    cases hx; rename_i hx
+    cases hx; rename_i hx
+    cases hx
+
+abbrev Ex4 := Expr.deref "l1"
+theorem Ex4.P : ∀ n, ¬Ex4.FV n := fun x hx => by cases hx
+
+end Q19
+
+theorem BvarShift.gen (hMain : TySpec Γ (Γ₂ ++ Γ') body tout)
+    : TySpec Γ (Γ₂ ++ Γlead ++ Γ') (body.bvarShift Γlead.length Γ₂.length) tout :=
+  match body with
+  | .bool b => by
+    cases hMain
+    exact .bool
+  | .int i => by
+    cases hMain
+    exact .int
+  | .skip => by
+    cases hMain
+    exact .skip
+  | .op lhs .add rhs => by
+    cases hMain
+    rename_i lhsIh rhsIh
+    exact .op_add (BvarShift.gen lhsIh) (BvarShift.gen rhsIh)
+  | .op lhs .gte rhs => by
+    cases hMain
+    rename_i lhsIh rhsIh
+    exact .op_gte (BvarShift.gen lhsIh) (BvarShift.gen rhsIh)
+  | .eif cond t f => by
+    cases hMain
+    rename_i condIh tIh fIh
+    exact .eif (BvarShift.gen condIh) (BvarShift.gen tIh) (BvarShift.gen fIh)
+  | .ewhile cond e => by
+    cases hMain
+    rename_i condIh eIh
+    exact .ewhile (BvarShift.gen condIh) (BvarShift.gen eIh)
+  | .assign addr e => by
+    cases hMain
+    rename_i p eIh
+    exact .assign p (BvarShift.gen eIh)
+  | .deref addr => by
+    cases hMain
+    exact .deref (by assumption)
+  | .seq a b => by
+    cases hMain
+    rename_i aIh bIh
+    exact .seq (BvarShift.gen aIh) (BvarShift.gen bIh)
+  | .bvar idx => by
+    cases hMain; case ref p =>
+    dsimp [Expr.bvarShift]
+    split
+    <;> rename_i x
+    · rw [List.append_assoc]
+      rw [List.getElem?_append x] at p
+      exact .ref (by rwa [List.getElem?_append x])
+    · simp only [not_lt] at x
+      rw [List.getElem?_append_right x] at p
+      exact .ref (by
+      rw [List.append_assoc, List.getElem?_append_right (Nat.le_add_right_of_le x)]
+      have h : Γlead.length ≤ idx + Γlead.length - Γ₂.length := by omega
+      rwa [
+        List.getElem?_append_right h,
+        Nat.sub_right_comm,
+        Nat.add_sub_assoc (Nat.le_refl _) _,
+        Nat.sub_self
+      ])
+  | .abs ty body => by
+    cases hMain
+    rename_i _ bodyIh
+    change TySpec _ (ty :: Γ₂ ++ Γ') _ _ at bodyIh
+    exact .abs (BvarShift.gen bodyIh)
+  | .app fn arg => by
+    cases hMain
+    rename_i argIh fnIh
+    exact .app (BvarShift.gen fnIh) (BvarShift.gen argIh)
+  | .letVal t' val body => by
+    cases hMain
+    rename_i valIh bodyIh
+    change TySpec _ (t' :: Γ₂ ++ Γ') _ _ at bodyIh
+    exact .letVal (BvarShift.gen valIh) (BvarShift.gen bodyIh)
+  | .letRecVal _ val body => by
+    cases hMain; next valIh bodyIh =>
+    change TySpec _ (_ :: Γ₂ ++ Γ') _ _ at bodyIh
+    change TySpec _ (_ :: _ :: Γ₂ ++ Γ') _ _ at valIh
+    exact .letRecValFn (BvarShift.gen valIh) (BvarShift.gen bodyIh)
+
+
+theorem Subst.gen (hTy : TySpec Γ Γ' e t) (hMain : TySpec Γ (Γlead ++ (t :: Γ')) body tout)
+    : TySpec Γ (Γlead ++ Γ') (body.replace Γlead.length e) tout :=
+  match body with
+  | .bool b => by
+    cases hMain
+    exact .bool
+  | .int i => by
+    cases hMain
+    exact .int
+  | .skip => by
+    cases hMain
+    exact .skip
+  | .op lhs .add rhs => by
+    cases hMain
+    rename_i lhsIh rhsIh
+    exact .op_add (Subst.gen hTy lhsIh) (Subst.gen hTy rhsIh)
+  | .op lhs .gte rhs => by
+    cases hMain
+    rename_i lhsIh rhsIh
+    exact .op_gte (Subst.gen hTy lhsIh) (Subst.gen hTy rhsIh)
+  | .eif cond t f => by
+    cases hMain
+    rename_i condIh tIh fIh
+    exact .eif (Subst.gen hTy condIh) (Subst.gen hTy tIh) (Subst.gen hTy fIh)
+  | .ewhile cond e => by
+    cases hMain
+    rename_i condIh eIh
+    exact .ewhile (Subst.gen hTy condIh) (Subst.gen hTy eIh)
+  | .assign addr e => by
+    cases hMain
+    rename_i p eIh
+    exact .assign p (Subst.gen hTy eIh)
+  | .deref addr => by
+    cases hMain
+    exact .deref (by assumption)
+  | .seq a b => by
+    cases hMain
+    rename_i aIh bIh
+    exact .seq (Subst.gen hTy aIh) (Subst.gen hTy bIh)
+  | .bvar idx => by
+    cases hMain; case ref p =>
+    dsimp [Expr.replace, Expr.replace.bvar]
+    split
+    <;> rename_i x
+    <;> simp only [Nat.compare_eq_eq, Nat.compare_eq_lt, Nat.compare_eq_gt] at x
+    · exact .ref (by rwa [List.getElem?_append x] at p ⊢)
+    · subst x
+      rw [List.getElem?_append_right (Nat.le_refl _), Nat.sub_self, List.getElem?_cons_zero, Option.some.injEq] at p
+      subst p
+      exact BvarShift.gen (Γ₂ := []) hTy
+    · refine .ref ?_
+      rw [List.getElem?_append_right (Nat.le_of_succ_le x)] at p
+      rw [List.getElem?_append_right (Nat.le_sub_one_of_lt x), Nat.sub_right_comm]
+      change ([_] ++ _)[_]? = _ at p
+      have : [t].length ≤ idx - Γlead.length := Nat.le_sub_of_add_le' x
+      rwa [List.getElem?_append_right this] at p
+  | .abs ty body => by
+    cases hMain
+    rename_i _ bodyIh
+    change TySpec _ (ty :: Γlead ++ t :: Γ') _ _ at bodyIh
+    exact .abs (Subst.gen hTy bodyIh)
+  | .app fn arg => by
+    cases hMain
+    rename_i argIh fnIh
+    exact .app (Subst.gen hTy fnIh) (Subst.gen hTy argIh)
+  | .letVal t' val body => by
+    cases hMain
+    rename_i valIh bodyIh
+    change TySpec _ (t' :: Γlead ++ t :: Γ') _ _ at bodyIh
+    exact .letVal (Subst.gen hTy valIh) (Subst.gen hTy bodyIh)
+  | .letRecVal _ val body => by
+    cases hMain; next valIh bodyIh =>
+    change TySpec _ (_ :: Γlead ++ t :: Γ') _ _ at bodyIh
+    change TySpec _ (_ :: _ :: Γlead ++ t :: Γ') _ _ at valIh
+    exact .letRecValFn (Subst.gen hTy valIh) (Subst.gen hTy bodyIh)
+
+theorem Subst : TySpec Γ Γ' e t → TySpec Γ (t :: Γ') body tout → TySpec Γ Γ' (body.replace 0 e) tout
+  := Subst.gen (Γlead := [])
+
+
+theorem TypePreservation (tyPre : TySpec Γ Γ' e t) (hMain : Red ⟨e, s1⟩ ⟨e', s2⟩) : TySpec Γ Γ' e' t :=
+  match e with
+  | .bool b => by
+    cases hMain
+  | .int i => by
+    cases hMain
+  | .skip => by
+    cases hMain
+  | .op lhs .add rhs => by
+    cases hMain <;> cases tyPre
+    · exact .int
+    case op1 ha lhs rhs =>
+      exact .op_add (TypePreservation lhs ha) rhs
+    case op2 hb lhs rhs => 
+      exact .op_add lhs (TypePreservation rhs hb)
+  | .op lhs .gte rhs => by
+    cases hMain <;> cases tyPre
+    · exact .bool
+    case op1 ha lhs rhs =>
+      exact .op_gte (TypePreservation lhs ha) rhs
+    case op2 hb lhs rhs => 
+      exact .op_gte lhs (TypePreservation rhs hb)
+  | .eif cond t f => by
+    cases hMain <;> cases tyPre
+    case if_t => assumption
+    case if_f => assumption
+    case if_cond ha cond t f =>
+      exact .eif (TypePreservation cond ha) t f
+  | .ewhile cond e =>
+    match tyPre with
+    | .ewhile cond e => by
+      cases hMain
+      obtain rfl : t = .void := by
+        cases tyPre
+        rfl
+      exact .eif cond (.seq e tyPre) .skip
+  | .assign addr e => by
+    cases hMain <;> cases tyPre
+    · exact .skip
+    case assign ha z ty =>
+      exact .assign z (TypePreservation ty ha)
+  | .deref addr => by
+    cases hMain
+    cases tyPre
+    exact .int
+  | .seq a b => by
+    cases hMain <;> cases tyPre
+    · assumption
+    case seq ha tya tyb =>
+      exact .seq (TypePreservation tya ha) tyb
+  | .bvar idx => by
+    cases hMain
+  | .abs ty body => by
+    cases hMain
+    /- rename_i _ bodyIh -/
+    /- change TySpec _ (ty :: Γlead ++ t :: Γ') _ _ at bodyIh -/
+    /- exact .abs (Subst.gen hTy bodyIh) -/
+  | .app fn arg => by
+    cases hMain <;> cases tyPre
+    case app1 ha _ argTy bodyTy =>
+      exact .app (TypePreservation bodyTy ha) argTy
+    case app2  ha _ argTy bodyTy =>
+      exact .app bodyTy (TypePreservation argTy ha)
+    case fn argTy bodyTy =>
+      cases bodyTy; next bodyTy =>
+      exact Subst argTy bodyTy
+  | .letVal t' val body => by
+    cases hMain <;> cases tyPre
+    case let1 ha argTy bodyTy => exact .letVal (TypePreservation argTy ha) bodyTy
+    case let2 argTy bodyTy =>
+      exact Subst argTy bodyTy
+  | .letRecVal _ val body => by
+    cases hMain
+
+/-- info: 'L2.TypePreservation' depends on axioms: [propext, Classical.choice, Quot.sound] -/
+#guard_msgs in #print axioms TypePreservation 
+
